

205040374 丁子豪 HW5.

1. Solution. Denote all the sets in each question as S .

(a) Given S_1 and S_2 are convex:

$$\forall x_{11}, x_{12} \in S_1. \quad \forall \lambda_1 \in [0, 1] \quad \lambda_1 x_{11} + (1 - \lambda_1) x_{12} \in S_1.$$

$$\forall x_{21}, x_{22} \in S_2. \quad \forall \lambda_2 \in [0, 1] \quad \lambda_2 x_{21} + (1 - \lambda_2) x_{22} \in S_2$$

$$\Rightarrow \forall y_1, y_2 \in S. \quad \exists y_{11}, y_{21} \in S_1. \quad y_{11}, y_{22} \in S_2$$

$$\text{S.t. } y_1 = y_{11} + y_{12}, \quad y_2 = y_{21} + y_{22}$$

$$\forall \lambda \in [0, 1] \quad \lambda y_1 + (1 - \lambda) y_2 = \lambda y_{11} + (1 - \lambda) y_{21} + \lambda y_{12} + (1 - \lambda) y_{22}$$

$$\text{Denote } z_1 = \lambda y_{11} + (1 - \lambda) y_{21}$$

$$z_2 = \lambda y_{12} + (1 - \lambda) y_{22}$$

$$\Rightarrow z_1 \in S_1. \quad z_2 \in S_2 \quad \text{Then } z_1 + z_2 \in S.$$

So S is convex.

(b). For $ax^2 + 2x + \frac{1}{a}$. $\Delta = 2^2 - 4 \cdot a \cdot \frac{1}{a} = 0$.

Given $a > 0$. $\forall x \in \mathbb{R}$. $ax^2 + 2x + \frac{1}{a} \geq 0$.

\mathbb{R} is convex i.e. $\forall x_1, x_2 \in \mathbb{R}$. $\lambda x_1 + (1-\lambda)x_2 \in \mathbb{R}$

Then the set is convex

(c). f is a convex function :

$$\forall x_1, x_2, \forall \lambda \in [0, 1]. f(\lambda x_1 + (1-\lambda)x_2) \leq \lambda f(x_1) + (1-\lambda)f(x_2)$$

$$\Rightarrow \forall s_1 = (y_1, x_1), s_2 = (y_2, x_2) \in S$$

$$y_1 \geq f(x_1), y_2 \geq f(x_2)$$

$$\lambda y_1 + (1-\lambda)y_2 \geq \lambda f(x_1) + (1-\lambda)f(x_2) \geq f(\lambda x_1 + (1-\lambda)x_2)$$

$$\text{Then } \lambda s_1 + (1-\lambda)s_2 = (\lambda y_1 + (1-\lambda)y_2, \lambda x_1 + (1-\lambda)x_2) \in S.$$

$\Rightarrow S$ is convex.

(d). Similar to (c).

$$\forall s_1 = (y_1, x_1), s_2 = (y_2, x_2) \in S \quad \forall \lambda \in [0, 1].$$

$$y_1 = f(x_1), \quad y_2 = f(x_2)$$

$$\lambda y_1 + (1-\lambda)y_2 = \lambda f(x_1) + (1-\lambda)f(x_2) \geq f(\lambda x_1 + (1-\lambda)x_2)$$

Then S is convex only when f is linear function

(e) Define $B = \frac{1}{2}(A + A^T)$. $\Rightarrow S = \{x \in \mathbb{R}^3; x^T B x \leq 0\}$.

$$B = \begin{pmatrix} 2 & -1 & 4 \\ -1 & 3 & 2 \\ 4 & 2 & -5 \end{pmatrix}$$

Sequential principal minors
of B are

$$M_1 = 2 > 0$$

$$M_2 = 5 > 0$$

$$M_3 = \det(B) = -97 < 0$$

So B is an indefinite matrix. S is not convex.

2. Solution

$$(a) \quad \forall x_1, x_2, \forall \lambda \in [0, 1].$$

$$\begin{aligned} f(\lambda x_1 + (1-\lambda)x_2) &= \sum_{i=1}^d |\lambda x_{1i} + (1-\lambda)x_{2i}| \\ &\leq \sum_{i=1}^d |\lambda x_{1i}| + |(1-\lambda)x_{2i}| \\ &= \lambda \sum_{i=1}^d |x_{1i}| + (1-\lambda) \sum_{i=1}^d |x_{2i}| \\ &= \lambda f(x_1) + (1-\lambda)f(x_2) \end{aligned}$$

So $f(x)$ is convex.

$$(b). \quad \forall x_1, x_2 \in \mathbb{R}^d, \forall \lambda \in [0, 1].$$

$$\begin{aligned} f(\lambda x_1 + (1-\lambda)x_2) &= \sum_{i=1}^d f_i(\lambda x_1 + (1-\lambda)x_2) \\ &\leq \sum_{i=1}^d \lambda f_i(x_1) + (1-\lambda)f_i(x_2) \\ &= \lambda f(x_1) + (1-\lambda)f(x_2) \end{aligned}$$

So $f(x)$ is convex.

(c). $\forall x_1, x_2 \in \mathbb{R}^d. \forall \mu \in [0, 1].$

$$\begin{aligned} f(\mu x_1 + (1-\mu)x_2) &\leq f(\mu x_1) + f((1-\mu)x_2) \\ &= \mu f(x_1) + (1-\mu)f(x_2) \\ &= \mu f(x_1) + (1-\mu)f(x_2). \end{aligned}$$

So $f(x)$ is convex.

(d). $f(x)$ is symmetric by axis y .

Consider $g(x) = x^{3/2}, x \geq 0.$

$$\frac{dg(x)}{dx} = \frac{3}{2} x^{1/2} \geq 0. \quad \frac{d^2g(x)}{dx^2} = \frac{3}{4} x^{-1/2} \geq 0.$$

$g(x)$ is convex so does $f(x)$.

(e). $x + \sqrt{1+x^2} \geq 0 \Leftrightarrow x \in \mathbb{R}.$

$$\frac{d f(x)}{dx} = \frac{1}{\sqrt{1+x^2}} + 2x. \quad \frac{d^2 f(x)}{dx^2} = 2 - x(1+x^2)^{-\frac{3}{2}}$$

$$2 - x(1+x^2)^{-\frac{3}{2}} \geq 0 \Leftrightarrow \frac{x}{(1+x^2)^{3/2}} \leq 2$$

$$\Leftrightarrow x \leq 2(1+x^2)^{3/2}$$

$$\Leftrightarrow x^2 \leq 4(1+x^2)^3$$

$$\forall x \in \mathbb{R}. x^2 \leq 4(1+x^2) \quad \text{So} \quad \frac{d^2 f(x)}{dx^2} \geq 0.$$

$f(x)$ is convex.

b. Solution.

$$\begin{aligned} (a). \quad f(\beta_0, \beta) &= \sum_{i=1}^n (\beta_0 + \beta^T x_i - y_i)^2 \\ &= \sum_{i=1}^n \beta_0^2 + 2\beta_0(\beta^T x_i - y_i) + (\beta^T x_i - y_i)^2 \\ &= n\beta_0^2 + 2\beta_0\left(\sum_{i=1}^n \beta^T x_i - \sum_{i=1}^n y_i\right) + \sum_{i=1}^n (\beta^T x_i - y_i)^2 \\ &= n\beta_0^2 + \sum_{i=1}^n (\beta^T x_i - y_i)^2 \end{aligned}$$

For $n\beta_0^2 \geq 0$. to minimize $f(x)$. β_0^* must be 0.

1b). To minimize $f(x)$. $\beta_0^* \geq 0$. β^* minimizes $(\beta^T x_i - y_i)^2$.

$$\begin{aligned}\tilde{f}(\beta_0, \beta) &= \sum_{i=1}^n (\beta_0 + \beta^T x_i' - y_i')^2 \\ &= \sum_{i=1}^n \beta_0^2 + 2\beta_0(\beta^T x_i' - y_i') + (\beta^T x_i' - y_i')^2 \\ &= n\beta_0^2 + 2\beta_0\left(\sum_{i=1}^n \beta^T x_i' - \sum_{i=1}^n y_i'\right) + \sum_{i=1}^n (\beta^T x_i' - y_i')^2\end{aligned}$$

we have: $\sum_{i=1}^n \beta^T x_i' = n\beta^T \bar{x}$. $\sum_{i=1}^n y_i' = n\bar{y}$

$$\Rightarrow \tilde{f}(\beta_0, \beta) = n\beta_0^2 + 2n\beta_0(\beta^T \bar{x} - \bar{y}) + \sum_{i=1}^n (\beta^T x_i' - y_i')^2$$

to minimize $g(\beta_0) = n\beta_0^2 + 2n\beta_0(\beta^T \bar{x} - \bar{y})$

$$\beta_0 = -\frac{2n(\beta^T \bar{x} - \bar{y})}{2n} = -\beta^T \bar{x} + \bar{y}.$$

$$\Rightarrow \beta_0 = \beta_0^* - \beta^T \bar{x} + \bar{y} \quad g(\beta_0) = -n\beta_0^2 = -n(\beta^T \bar{x} - \bar{y})^2.$$

WITH best β_0 .

$$\begin{aligned}\tilde{f}(\beta_0, \beta) &= \sum_{i=1}^n (\beta^T x_i' - y_i')^2 - (\beta^T z - r)^2 \\&= \sum_{i=1}^n (\beta^T x_i' - y_i' - \beta^T z + r)(\beta^T x_i' - y_i' + \beta^T z - r) \\&= \sum_{i=1}^n (\beta^T x_i - y_i)(\beta^T x_i - y_i + 2\beta^T z - 2r) \\&= \sum_{i=1}^n (\beta^T x_i - y_i)^2 + 2\beta_0 (\beta^T x_i - y_i) \\&= \sum_{i=1}^n (\beta^T x_i - y_i)^2 + 2\beta_0 \left(\sum_{i=1}^n \beta^T x_i - \sum_{i=1}^n y_i \right) \\&= \sum_{i=1}^n (\beta^T x_i - y_i)^2\end{aligned}$$

As β^* minimizes $(\beta^T x_i - y_i)^2$. here $\beta = \beta^*$.

So the statement holds for $f(\beta_0, \beta)$ and $\tilde{f}(\beta_0, \beta)$.

4. Solution

(a) ① Objective function $f(x_1, x_2)$

$$\frac{\partial}{\partial x_1} f(x_1, x_2) = 6x_1 + 2x_2$$

$$\frac{\partial}{\partial x_2} f(x_1, x_2) = 2x_1 + 8x_2$$

$$\Rightarrow \nabla^2 f(x_1, x_2) = \begin{pmatrix} 6 & 2 \\ 2 & 8 \end{pmatrix} \text{ is p.d.}$$

\Rightarrow Objective function is convex.

② Constraint $g(x_1, x_2) = (1 + x_1^2 + x_2^2)^{1/2} + x_1$

$$\frac{\partial}{\partial x_1} g(x_1, x_2) = x_1(1 + x_1^2 + x_2^2)^{-1/2} + 1$$

$$\frac{\partial}{\partial x_2} g(x_1, x_2) = x_2(1 + x_1^2 + x_2^2)^{-1/2}$$

$$\nabla^2 g(x_1, x_2) = \begin{pmatrix} (1 + x_1^2 + x_2^2)^{-1/2} - x_1^2(1 + x_1^2 + x_2^2)^{-3/2}, & -x_1x_2(1 + x_1^2 + x_2^2)^{-3/2} \\ -x_1x_2(1 + x_1^2 + x_2^2)^{-3/2}, & (1 + x_1^2 + x_2^2)^{-1/2} - x_2^2(1 + x_1^2 + x_2^2)^{-3/2} \end{pmatrix}$$

$$= (1+x_1^2+x_2^2)^{-\frac{3}{2}} \begin{pmatrix} 1+x_2^2 & -x_1x_2 \\ -x_1x_2 & 1+x_1^2 \end{pmatrix}$$

$$\text{For } A = \begin{pmatrix} 1+x_2^2 & -x_1x_2 \\ -x_1x_2 & 1+x_1^2 \end{pmatrix}$$

$$M_1 = 1+x_2^2 > 0.$$

$$M_2 = (1+x_1^2)(1+x_2^2) - x_1^2x_2^2 = 1+x_1^2+x_2^2 > 0.$$

$\Rightarrow g(x_1, x_2)$ is convex.

So this is a convex problem.

(b). Lagrangian function:

$$L(x_1, x_2, \lambda) = 3x_1^2 + 4x_2^2 + 2x_1x_2 + \lambda [(1+x_1^2+x_2^2)^{\frac{1}{2}} + x_1 - 2]$$

KKT condition: ① $(1+x_1^2+x_2^2)^{\frac{1}{2}} + x_1 - 2 \leq 0.$

$$\text{② } \lambda \geq 0.$$

$$\text{③ } \nabla_1 L = 6x_1 + 2x_2 + \lambda [x_1(1+x_1^2+x_2^2)^{-\frac{1}{2}} + 1] = 0.$$

$$\nabla_2 L = 2x_1 + 8x_2 + \lambda x_2(1+x_1^2+x_2^2)^{-\frac{1}{2}} = 0.$$

$$(4) \quad \lambda [(1+x_1^2+x_2^2)^{1/2} + x_1 - 2] = 0.$$

$$x_1 \nabla_1 L = 0.$$

$$x_2 \nabla_2 L = 0.$$

10). 1). $\lambda = 0$. $\nabla_1 L = 6x_1 + 2x_2 = 0$. $\Rightarrow (x_1, x_2, \lambda) = (0, 0, 0)$.
 $\nabla_2 L = 2x_1 + 8x_2 = 0$.

2). $\lambda > 0$. $(1+x_1^2+x_2^2)^{1/2} + x_1 - 2 = 0$.

$$\nabla_1 L = 6x_1 + 2x_2 + \lambda [x_1 (1+x_1^2+x_2^2)^{-1/2} + 1] = 0.$$

$$\nabla_2 L = 2x_1 + 8x_2 + \lambda x_2 (1+x_1^2+x_2^2)^{-1/2} = 0.$$

Denote $y = (1+x_1^2+x_2^2)^{-1/2} > 0$.

$$\Rightarrow \nabla_1 L = 6x_1 + 2x_2 + \lambda (x_1 y + 1) = 0.$$

$$\nabla_2 L = 2x_1 + 8x_2 + \lambda x_2 y = 0.$$

Also. $y + x_1 - 2 = 0$. $y = \frac{1}{x_1 - 2}$

The equations do not have solutions.

$$\Rightarrow \text{KKT point is } (0, 0)$$